> [!Question]
> 1. $\lim\limits_{ x \to 1 } \dfrac{x^\sqrt{ 2 } - 1}{x^2 - 1}$
> 2. $\lim\limits_{ x \to 0 } \left( \dfrac{3^x + 5^x + 7^x}{3} \right)^{1/x}$
> 3. $\lim\limits_{ n \to \infty }\sum\limits_{ k = 1 }^{ 2n } \dfrac{1}{n+k}$
> 4. $\lim\limits_{ n \to \infty } \prod\limits_{k=1}^{n}\left( 1+\dfrac{k}{n^2} \right)$



> [!Question]
> 求证$x_{n} = \sum\limits_{ k = 1 }^{ n } \dfrac{\sin k}{k^2}$收敛。



> [!Question]
> 连续函数$f(x)$满足$f(x)+f(y) = f(x+y)$，求$f(x)$的表达式。



> [!Question]
> $f(x), g(x): (-\infty, +\infty) \to \mathbb{R}$ 且均为周期函数且 $\lim\limits_{ x \to +\infty } (f(x) - g(x)) = 0$，求证：$f, g$ 具有相同的周期

> [!Proof]
> $|g(x + T) - g(x)| \leq |g(x + T) - f(x + T)| + |f(x + T) - f(x)| + |f(x) - g(x)|$ 其中 $T$ 是 $f$ 的周期， 则
> $$\lim\limits_{ x \to +\infty }(g(x + T) - g(x)) = 0$$
> 反证，假设$\exists a$使得$g(a+T)-g(a) \neq 0$。设$T'$是$g(x)$的周期，则
> $$g(a+T+nT')-g(a+nT') = g(a+T) - g(a)$$
> 两边令$n \to +\infty$，得
> $$0 = g(a+T) - g(a)$$
> 矛盾







